03: finish 3.5.16

03-untyped/03Untyped/Basic.lean
@@ -256,30 +256,283 @@ theorem value_is_normal : Value v → Normal v := by
 def Stuck : Term → Prop
 | t => Normal t ∧ ¬ Value t
 
-inductive BigStep : Term → Term → Prop
-| Value : Value v → BigStep v v
--- Do we need Value v in those two cases below?
-| IfTrue : Value v → BigStep c Term.True → BigStep t v → BigStep (Term.If c t e) v
-| IfFalse : Value v → BigStep c Term.False → BigStep e v → BigStep (Term.If c t e) v
-| Succ : NatV v → BigStep t v → BigStep (Term.Succ t) (Term.Succ v)
-| PredZero : BigStep t Term.Zero → BigStep (Term.Pred t) Term.Zero
-| PredSucc : NatV v → BigStep t (Term.Succ v) → BigStep (Term.Pred t) v
-| IsZeroZero : BigStep t Term.Zero → BigStep (Term.IsZero t) Term.True
-| IsZeroSucc : NatV v → BigStep t (Term.Succ v) → BigStep (Term.IsZero t) Term.False
-
-theorem step_implies_big_step : Value v → Step t t' → BigStep t v → BigStep t' v := by
-  intro hv hs hbs
-  unhygienic induction t generalizing t' v <;>
-  { grind (splits := 20) [BigStep, Value, NatV, Step] }
-
-theorem big_step_implies_step : Value v → Step t' t → BigStep t v → BigStep t' v := by
-  intro hv hs hbs
-  unhygienic induction t generalizing t' v <;>
-  { grind (splits := 20) [BigStep, Value, NatV, Step] }
+theorem aug_multi_step : ∀ f : Term → Term,
+  (∀ t t', (Step t t' → Step (f t) (f t'))) →
+  MultiStep t t' → MultiStep (f t) (f t') := by
+  intro f hf ht
+  induction ht <;> grind [MultiStep]
 
 theorem multi_step_trans : MultiStep t t' → MultiStep t' t'' → MultiStep t t'' := by
   intro h
   induction h <;> grind [MultiStep]
+
+inductive WTerm
+| True : WTerm
+| False : WTerm
+| If (c t e : WTerm) : WTerm
+| Zero : WTerm
+| Succ (t : WTerm) : WTerm
+| Pred (t : WTerm) : WTerm
+| IsZero (t : WTerm) : WTerm
+| Wrong
+
+def Eqt : WTerm → Term → Prop
+| .True, .True => True
+| .False, .False => True
+| .If c₁ t₁ e₁, .If c t e => Eqt c₁ c ∧ Eqt t₁ t ∧ Eqt e₁ e
+| .Zero, .Zero => True
+| .Succ t₁, .Succ t₂ => Eqt t₁ t₂
+| .Pred t₁, .Pred t₂ => Eqt t₁ t₂
+| .IsZero t₁, .IsZero t₂ => Eqt t₁ t₂
+| .Wrong, _ => False
+| _, _ => False
+
+inductive BadNat : WTerm → Prop
+| BadTrue : BadNat (.True)
+| BadFalse : BadNat (.False)
+| BadWrong : BadNat (.Wrong)
+
+inductive BadBool : WTerm → Prop
+| BadSucc : BadBool (.Succ v)
+| BadZero : BadBool (.Zero)
+| BadWrong : BadBool (.Wrong)
+
+inductive WStep : WTerm → WTerm → Prop
+| IfTrue : WStep (.If .True t e) t
+| IfFalse : WStep (.If .False t e) e
+| IfStep : WStep c c' → WStep (.If c t e) (.If c' t e)
+| SuccStep : WStep t t' → WStep (.Succ t) (.Succ t')
+| PredZero : WStep (.Pred .Zero) .Zero
+| PredSucc : Eqt t₁ t₂ → NatV t₂ → WStep (.Pred (.Succ t₁)) t₁
+| PredStep : WStep t t' → WStep (.Pred t) (.Pred t')
+| IsZeroZero : WStep (.IsZero .Zero) .True
+| IsZeroSucc : Eqt t₁ t₂ → NatV t₂ → WStep (.IsZero (.Succ t₁)) .False
+| IsZeroStep : WStep t t' → WStep (.IsZero t) (.IsZero t')
+| IfBadBool : BadBool t → WStep (.If t p n) .Wrong
+| SuccWrong : BadNat t → WStep (.Succ t) .Wrong
+| PredWrong : BadNat t → WStep (.Pred t) .Wrong
+| IsZeroWrong : BadNat t → WStep (.IsZero t) .Wrong
+
+
+inductive WMultiStep : WTerm → WTerm → Prop
+| Refl : WMultiStep t t
+| Step : WStep t t' → WMultiStep t' t'' → WMultiStep t t''
+
+
+def WNormal : WTerm → Prop
+| t => ¬ ∃ t', WStep t t'
+
+theorem stuck_if : Stuck (Term.If t p n) → (Stuck t ∨ NatV t) := by
+  unfold Stuck Normal
+  simp only [not_exists, and_imp]
+  intro hx hv
+  by_cases hnv : NatV t
+  { simp [hnv] }
+  simp only [hnv, or_false]
+  constructor
+  { intro x stx
+    have := Step.IfStep stx (t := p) (e := n)
+    grind [Step] }
+  intro hvt
+  cases hvt
+  { have := Step.IfTrue (t := p) (e := n)
+    grind }
+  { have := Step.IfFalse (t := p) (e := n)
+    grind }
+  grind [Stuck, Normal, Value, Step]
+
+theorem stuck_succ : Stuck (Term.Succ t) → (Stuck t ∨ t = .False ∨ t = .True) := by
+  unfold Stuck Normal
+  simp only [not_exists, and_imp]
+  intro hx hv
+  by_cases hnv : t = Term.False ∨ t = Term.True
+  { simp [hnv] }
+  simp only [hnv, or_false]
+  constructor
+  { intro x stx
+    have := Step.SuccStep stx
+    grind [Step] }
+  grind [Stuck, Normal, Value, Step, NatV]
+
+theorem stuck_pred : Stuck (Term.Pred t) → (Stuck t ∨ t = .False ∨ t = .True) := by
+  unfold Stuck Normal
+  simp only [not_exists, and_imp]
+  intro hx hv
+  by_cases hnv : t = Term.False ∨ t = Term.True
+  { simp [hnv] }
+  simp only [hnv, or_false]
+  constructor
+  { intro x stx
+    have := Step.PredStep stx
+    grind [Step] }
+  intro hvt
+  cases hvt
+  { grind }
+  { grind }
+  rename_i hvs
+  unhygienic cases hvs
+  { grind [Value, Step] }
+  have := Step.PredSucc a
+  grind [Stuck, Normal, Value, Step, NatV]
+
+theorem stuck_isZero : Stuck (Term.IsZero t) → (Stuck t ∨ t = .False ∨ t = .True) := by
+  unfold Stuck Normal
+  simp only [not_exists, and_imp]
+  intro hx hv
+  by_cases hnv : t = Term.False ∨ t = Term.True
+  { simp [hnv] }
+  simp only [hnv, or_false]
+  constructor
+  { intro x stx
+    have := Step.IsZeroStep stx
+    grind [Step] }
+  intro hvt
+  unhygienic cases hvt
+  { grind }
+  { grind }
+  unhygienic cases a
+  { grind [Step] }
+  have := Step.IsZeroSucc a_1
+  grind [Stuck, Normal, Value, Step, NatV]
+
+
+theorem aug_wmulti_step (t₁ t₂ : WTerm) : ∀ f : WTerm → WTerm,
+  (∀ t t', (WStep t t' → WStep (f t) (f t'))) →
+  WMultiStep t₁ t₂ → WMultiStep (f t₁) (f t₂) := by
+  intro f hf ht
+  induction ht <;> grind [WMultiStep]
+
+theorem multi_wstep_trans : WMultiStep t t' → WMultiStep t' t'' → WMultiStep t t'' := by
+  intro h
+  induction h <;> grind [WMultiStep]
+
+theorem stuck_is_wrong : Eqt t₁ t → Stuck t → WMultiStep t₁ .Wrong := by
+  intro eq st
+  unhygienic fun_induction Eqt
+  { grind [Stuck, Normal, Value, Step, WStep] }
+  { grind [Stuck, Normal, Value, Step, WStep] }
+  { unhygienic cases stuck_if st
+    { apply multi_wstep_trans
+      { apply aug_wmulti_step c₁ .Wrong (fun t₁ => t₁.If t₁_1 e₁) (by grind [WStep]) (by grind) }
+      apply WMultiStep.Step
+      { apply WStep.IfBadBool
+        grind [BadBool] }
+      grind [WMultiStep] }
+    have : BadBool c₁ := by
+      cases h
+      { have : c₁ = WTerm.Zero := by grind [Eqt]
+        grind [BadBool] }
+      { have : ∃ t1, c₁ = WTerm.Succ t1 := by
+          have str := eq.1
+          unfold Eqt at str
+          split at str
+          all_goals try grind
+        grind [BadBool] }
+    apply WMultiStep.Step
+    { apply WStep.IfBadBool
+      grind [BadBool] }
+    grind [WMultiStep] }
+  { grind [Stuck, Normal, Value, NatV] }
+  { unhygienic cases stuck_succ st
+    { apply multi_wstep_trans
+      { apply aug_wmulti_step t₁_1 .Wrong .Succ (by grind [WStep]) (by grind) }
+      apply WMultiStep.Step
+      { apply WStep.SuccWrong
+        grind [BadNat] }
+      grind [WMultiStep] }
+    cases h <;>
+    { have : t₁_1 = WTerm.False ∨ t₁_1 = WTerm.True := by grind [Eqt]
+      apply WMultiStep.Step
+      { apply WStep.SuccWrong
+        grind [WMultiStep, WStep, BadNat, Eqt] }
+      apply WMultiStep.Refl } }
+  { unhygienic cases stuck_pred st
+    { apply multi_wstep_trans
+      { apply aug_wmulti_step t₁_1 .Wrong .Pred (by grind [WStep]) (by grind) }
+      apply WMultiStep.Step
+      { apply WStep.PredWrong
+        grind [BadNat] }
+      grind [WMultiStep] }
+    cases h <;>
+    { have : t₁_1 = WTerm.False ∨ t₁_1 = WTerm.True := by grind [Eqt]
+      apply WMultiStep.Step
+      { apply WStep.PredWrong
+        grind [WMultiStep, WStep, BadNat, Eqt] }
+      apply WMultiStep.Refl } }
+  { unhygienic cases stuck_isZero st
+    { apply multi_wstep_trans
+      { apply aug_wmulti_step t₁_1 .Wrong .IsZero (by grind [WStep]) (by grind) }
+      apply WMultiStep.Step
+      { apply WStep.IsZeroWrong
+        grind [BadNat] }
+      grind [WMultiStep] }
+    cases h <;>
+    { have : t₁_1 = WTerm.False ∨ t₁_1 = WTerm.True := by grind [Eqt]
+      apply WMultiStep.Step
+      { apply WStep.IsZeroWrong
+        grind [WMultiStep, WStep, BadNat, Eqt] }
+      apply WMultiStep.Refl } }
+  { apply WMultiStep.Refl }
+  grind
+
+theorem step_is_wstep : Eqt t₁ t1 → (Step t1 t2) → ∃ t₂, (WStep t₁ t₂) ∧ Eqt t₂ t2 := by
+  intro eq st
+  unhygienic fun_induction Eqt generalizing t2
+  { exists WTerm.True }
+  { exists WTerm.False }
+  { unhygienic cases st
+    { have : c₁ = WTerm.True := by grind [Eqt]
+      exists t₁_1
+      grind [WStep] }
+    { have : c₁ = WTerm.False := by grind [Eqt]
+      exists e₁
+      grind [WStep] }
+    rcases ih3 (t2 := c') eq.1 a with ⟨t2, ht2⟩
+    exists t2.If t₁_1 e₁
+    grind [WStep, Eqt] }
+  { exists WTerm.Zero }
+  { unhygienic cases st
+    rcases ih1 (t2 := t') eq a with ⟨t₂, ht₂⟩
+    exists t₂.Succ
+    grind [WStep, Eqt] }
+  { unhygienic cases st
+    { exists WTerm.Zero
+      have : t₁_1 = WTerm.Zero := by grind [Eqt]
+      grind [Eqt, WStep] }
+    { have : ∃ t₁_2, t₁_1 = WTerm.Succ t₁_2 := by
+        unfold Eqt at eq
+        split at eq <;> try grind
+      rcases this with ⟨tval, htval⟩
+      rw [htval]
+      exists tval
+      grind [WStep, Eqt] }
+    rcases ih1 (t2 := t') eq a with ⟨t₂, ht₂⟩
+    exists t₂.Pred
+    grind [WStep, Eqt] }
+  { unhygienic cases st
+    { exists WTerm.True
+      have : t₁_1 = WTerm.Zero := by grind [Eqt]
+      grind [Eqt, WStep] }
+    { have : ∃ t₁_2, t₁_1 = WTerm.Succ t₁_2 := by
+        unfold Eqt at eq
+        split at eq <;> try grind
+      rcases this with ⟨tval, htval⟩
+      rw [htval]
+      exists WTerm.False
+      grind [WStep, Eqt] }
+    rcases ih1 (t2 := t') eq a with ⟨t₂, ht₂⟩
+    exists t₂.IsZero
+    grind [WStep, Eqt] }
+  { grind }
+  grind
+
+theorem eq_det (t1 : WTerm) (t2 t3 : Term) : Eqt t1 t2 → Eqt t1 t3 → t2 = t3 := by
+  intro eq
+  unhygienic fun_induction Eqt t1 t2 generalizing t3 <;> try grind [Eqt]
+  all_goals {
+    intro eq1
+    unfold Eqt at eq1
+    split at eq1 <;> grind }
 
 def size : Term → Nat
 | .True => 1
@@ -301,6 +554,244 @@ theorem multi_step_size : MultiStep t t' → size t > size t' ∨ t = t' := by
   cases a_ih <;>
   { have step_sz := step_size a
     grind [step_size] }
+
+
+def wsize : WTerm → Nat
+| .True => 1
+| .False => 1
+| .If (c : WTerm) (t : WTerm) (e : WTerm) => 1 + wsize c + wsize t + wsize e
+| .Zero => 1
+| .Succ (t : WTerm) => 1 + wsize t
+| .Pred (t : WTerm) => 1 + wsize t
+| .IsZero (t : WTerm) => 1 + wsize t
+| .Wrong => 1
+
+theorem wstep_size : WStep t t' → wsize t > wsize t' := by
+  intro h
+  unhygienic induction h <;> try grind [wsize, BadBool, BadNat]
+
+theorem multi_steps_finishes (t : Term) : ∃ t', MultiStep t t' ∧ Normal t' := by
+  by_cases ht : Normal t
+  { grind [MultiStep] }
+  unfold Normal at ht
+  have : ∃ t', Step t t' := by grind
+  rcases this with ⟨t', ht'⟩
+  rcases multi_steps_finishes t' with ⟨t1, ht1⟩
+  grind [MultiStep]
+termination_by size t
+decreasing_by
+  apply step_size
+  apply ht'
+
+theorem multi_steps_multi_wsteps (t t1 : Term) (t2 : WTerm) :
+  Eqt t2 t → MultiStep t t1 → ∃ t3, WMultiStep t2 t3 ∧ Eqt t3 t1 := by
+    intro eq hms
+    unhygienic cases hms
+    { grind [WMultiStep] }
+    rcases step_is_wstep eq a with ⟨t3, ht3⟩
+    rcases multi_steps_multi_wsteps t' t1 t3 ht3.2 a_1 with ⟨t4, ht4⟩
+    exists t4
+    simp [ht4]
+    grind [WMultiStep]
+termination_by size t
+decreasing_by
+  apply step_size
+  grind
+
+
+theorem wstep_preserves_badbool (t1 t2 : WTerm) :
+  WStep t1 t2 → BadBool t1 → BadBool t2 := by
+    grind [WStep, BadBool]
+
+theorem wterm_nat (t1 t2 : WTerm) (t : Term) :
+  WStep t1 t2 → NatV t → Eqt t1 t → False := by
+    intro hs hn heq
+    unhygienic cases hn
+    { have : t1 = .Zero := by grind [Eqt]
+      grind [WStep] }
+    have : ∃ t, WTerm.Succ t = t1 := by
+      unfold Eqt at heq
+      split at heq <;> grind
+    rcases this with ⟨t, ht⟩
+    unhygienic cases hs <;> try grind
+    { apply wterm_nat t_2 t' t_1 a_1 a (by grind [Eqt]) }
+    have : Eqt t_2 t_1 := by grind [Eqt]
+    unhygienic cases a_1
+    { have : t_1 = .True := by grind [Eqt]
+      grind [NatV] }
+    { have : t_1 = .False := by grind [Eqt]
+      grind [NatV] }
+    grind [WStep, NatV, Eqt, BadNat]
+
+
+theorem wstep_det (t1 t2 t3 : WTerm) :
+  WStep t1 t2 → WStep t1 t3 →
+  t2 = t3 ∨
+  WMultiStep t2 .Wrong ∧ WMultiStep t3 .Wrong := by
+    intro hs1 hs2
+    by_cases t2 = t3
+    { apply Or.inl
+      assumption }
+    apply Or.inr
+    unhygienic cases hs1 <;> unhygienic cases hs2 <;> try grind [WStep, BadBool, BadNat]
+    { unhygienic cases wstep_det c c' c'_1 a a_1
+      { grind }
+      constructor <;>
+      { apply multi_wstep_trans
+        { apply aug_wmulti_step (t₂ := .Wrong) (f := fun t4 => t4.If t e)
+          { grind [WStep] }
+          grind }
+        apply WMultiStep.Step
+        { apply WStep.IfBadBool
+          grind [WMultiStep, WStep, BadBool] }
+        apply WMultiStep.Refl } }
+    { constructor
+      { have : BadBool c' := by grind [wstep_preserves_badbool]
+        apply WMultiStep.Step
+        { apply WStep.IfBadBool
+          grind [WMultiStep, WStep] }
+        apply WMultiStep.Refl }
+      apply WMultiStep.Refl }
+    { unhygienic cases wstep_det t t' t'_1 a a_1
+      { grind }
+      constructor <;>
+      { apply multi_wstep_trans
+        { apply aug_wmulti_step (t₂ := .Wrong) (f := .Succ)
+          { grind [WStep] }
+          grind }
+        apply WMultiStep.Step
+        { apply WStep.SuccWrong
+          grind [WMultiStep, WStep, BadNat] }
+        apply WMultiStep.Refl } }
+    { unhygienic cases a_2
+      { grind [wterm_nat] }
+      cases a_3 <;> grind [Eqt, NatV] }
+    { unhygienic cases a
+      { grind [wterm_nat] }
+      cases a_3 <;> grind [Eqt, NatV] }
+    { unhygienic cases wstep_det t t' t'_1 a a_1
+      { grind }
+      constructor <;>
+      { apply multi_wstep_trans
+        { apply aug_wmulti_step (t₂ := .Wrong) (f := .Pred)
+          { grind [WStep] }
+          grind }
+        apply WMultiStep.Step
+        { apply WStep.PredWrong
+          grind [WMultiStep, WStep, BadNat] }
+        apply WMultiStep.Refl } }
+    { unhygienic cases a_2
+      { grind [wterm_nat] }
+      cases a_3 <;> grind [Eqt, NatV] }
+    { unhygienic cases a
+      { grind [wterm_nat] }
+      cases a_3 <;> grind [Eqt, NatV] }
+    { unhygienic cases wstep_det t t' t'_1 a a_1
+      { grind }
+      constructor <;>
+      { apply multi_wstep_trans
+        { apply aug_wmulti_step (t₂ := .Wrong) (f := .IsZero)
+          { grind [WStep] }
+          grind }
+        apply WMultiStep.Step
+        { apply WStep.IsZeroWrong
+          grind [WMultiStep, WStep, BadNat] }
+        apply WMultiStep.Refl } }
+    constructor
+    { apply WMultiStep.Refl }
+    apply WMultiStep.Step
+    { apply WStep.IfBadBool
+      have : BadBool c' := by grind [wstep_preserves_badbool]
+      grind [WMultiStep, WStep] }
+    apply WMultiStep.Refl
+termination_by wsize t1
+decreasing_by
+  all_goals grind [wstep_size, wsize]
+
+theorem multi_wstep_wrong (t1 t2 : WTerm) :
+  WMultiStep t1 t2 → WMultiStep t1 .Wrong → WMultiStep t2 .Wrong := by
+  intro h1 h2
+  unhygienic cases h1
+  { grind [WMultiStep, WStep] }
+  apply multi_wstep_wrong t' t2
+  { apply a_1 }
+  unhygienic cases h2
+  { grind [WMultiStep, WStep] }
+  unhygienic cases wstep_det t1 t' t'_1 a a_2
+  { grind }
+  exact h.1
+termination_by wsize t1
+decreasing_by
+  apply wstep_size
+  grind
+
+theorem multi_wstep_natv (t1 t2 : WTerm) (t : Term) :
+  WStep t1 t2 → NatV t → Eqt t1 t → False := by
+  intro hms eq hn
+  unhygienic cases eq
+  { have : t1 = .Zero := by grind [Eqt]
+    grind [Eqt, WStep] }
+  have : ∃ t3, WTerm.Succ t3 = t1 := by
+    unfold Eqt at hn
+    split at hn <;> grind
+  rcases this with ⟨t3, ht3⟩
+  have : Eqt t3 t_1 := by grind [Eqt]
+  unhygienic cases hms <;> try grind
+  { apply multi_wstep_natv t t' t_1 a_1 a (by grind [Eqt]) }
+  cases a_1 <;> grind [Eqt, NatV]
+
+theorem stuck_iff_wrong : Eqt t₁ t → (WMultiStep t₁ .Wrong ↔ ∃ t', MultiStep t t' ∧ Stuck t') := by
+  intro eq
+  constructor
+  { intro hwm
+    rcases multi_steps_finishes t with ⟨t1, ht1⟩
+    exists t1
+    simp only [ht1]
+    unfold Stuck
+    simp only [true_and, ht1]
+    intro hv
+    rcases multi_steps_multi_wsteps t t1 t₁ eq ht1.1 with ⟨t2, ht2⟩
+    have : WMultiStep t2 .Wrong  := by
+      apply multi_wstep_wrong t₁ t2 ht2.1 hwm
+    unhygienic cases hv
+    { have eq : t2 = .True := by grind [Eqt]
+      cases this
+      { grind }
+      grind [WStep] }
+    { have eq : t2 = .False := by grind [Eqt]
+      cases this
+      { grind }
+      grind [WStep] }
+    cases this
+    { grind [Eqt] }
+    grind [multi_wstep_natv] }
+  rintro ⟨t', ms, st⟩
+  unhygienic induction ms generalizing t₁
+  { apply stuck_is_wrong eq st }
+  rcases step_is_wstep eq a with ⟨t1, ht1⟩
+  have lem := a_ih (t₁ := t1) ht1.2 st
+  grind [WMultiStep]
+
+inductive BigStep : Term → Term → Prop
+| Value : Value v → BigStep v v
+-- Do we need Value v in those two cases below?
+| IfTrue : Value v → BigStep c Term.True → BigStep t v → BigStep (Term.If c t e) v
+| IfFalse : Value v → BigStep c Term.False → BigStep e v → BigStep (Term.If c t e) v
+| Succ : NatV v → BigStep t v → BigStep (Term.Succ t) (Term.Succ v)
+| PredZero : BigStep t Term.Zero → BigStep (Term.Pred t) Term.Zero
+| PredSucc : NatV v → BigStep t (Term.Succ v) → BigStep (Term.Pred t) v
+| IsZeroZero : BigStep t Term.Zero → BigStep (Term.IsZero t) Term.True
+| IsZeroSucc : NatV v → BigStep t (Term.Succ v) → BigStep (Term.IsZero t) Term.False
+
+theorem step_implies_big_step : Value v → Step t t' → BigStep t v → BigStep t' v := by
+  intro hv hs hbs
+  unhygienic induction t generalizing t' v <;>
+  { grind (splits := 20) [BigStep, Value, NatV, Step] }
+
+theorem big_step_implies_step : Value v → Step t' t → BigStep t v → BigStep t' v := by
+  intro hv hs hbs
+  unhygienic induction t generalizing t' v <;>
+  { grind (splits := 20) [BigStep, Value, NatV, Step] }
 
 theorem multi_step_if_eval_true : MultiStep t Term.True → MultiStep ((Term.If t) p n) p := by
   intro hv
@@ -328,12 +819,6 @@ theorem multi_step_if_eval_false : MultiStep t Term.False → MultiStep ((Term.I
   exact a_1
 termination_by size t
 decreasing_by exact step_size a
-
-theorem aug_multi_step : ∀ f : Term → Term,
-  (∀ t t', (Step t t' → Step (f t) (f t'))) →
-  MultiStep t t' → MultiStep (f t) (f t') := by
-  intro f hf ht
-  induction ht <;> grind [MultiStep]
 
 theorem big_step_is_multi_step : Value v → (BigStep t v ↔ MultiStep t v) := by
   intro hv
